wiring up parsing and desugaring with the main checker

pulse/src/ocaml/plugin/Pulse_Parser.ml
@@ -231,7 +231,7 @@ let parse_decl (s:string) (r:range) =
   let lexbuf, lexer = lexbuf_and_lexer s r in
   try
     let d = MenhirLib.Convert.Simplified.traditional2revised PP.pulseDecl lexer in
-    Inl r
+    Inl d
   with
   | e ->
     let pos = FStar_Parser_Util.pos_of_lexpos (lexbuf.cur_p) in
