pulse/src/ocaml/plugin/generated/PulseASTBuilder.ml
@@ -1,10 +1,11 @@
 open Prims
-let (r_ : FStar_Compiler_Range.range) = FStar_Compiler_Range.dummyRange
+let (r_ : FStar_Compiler_Range_Type.range) =
+  FStar_Compiler_Range_Type.dummyRange
 let (pulse_checker_tac : FStar_Ident.lident) =
   FStar_Ident.lid_of_path ["Pulse"; "Main"; "check_pulse"] r_
 let (tm :
   FStar_Parser_AST.term' ->
-    FStar_Compiler_Range.range -> FStar_Parser_AST.term)
+    FStar_Compiler_Range_Type.range -> FStar_Parser_AST.term)
   =
   fun t ->
     fun r ->
@@ -16,17 +17,26 @@ let (tm :
 let (extension_parser : FStar_Parser_AST_Util.extension_parser) =
   fun ctx ->
     fun contents ->
-      fun rng ->
-        let tm1 t = tm t rng in
+      fun r ->
+        let tm1 t = tm t r in
         let str s =
-          tm1 (FStar_Parser_AST.Const (FStar_Const.Const_string (s, rng))) in
-        let uu___ = Pulse_Parser.parse_peek_id contents rng in
+          tm1 (FStar_Parser_AST.Const (FStar_Const.Const_string (s, r))) in
+        let i s =
+          let uu___ =
+            let uu___1 =
+              let uu___2 =
+                let uu___3 = FStar_Compiler_Util.string_of_int s in
+                (uu___3, FStar_Pervasives_Native.None) in
+              FStar_Const.Const_int uu___2 in
+            FStar_Parser_AST.Const uu___1 in
+          tm1 uu___ in
+        let uu___ = Pulse_Parser.parse_peek_id contents r in
         match uu___ with
-        | FStar_Pervasives.Inr (err, r) ->
+        | FStar_Pervasives.Inr (err, r1) ->
             FStar_Pervasives.Inl
               {
                 FStar_Parser_AST_Util.message = err;
-                FStar_Parser_AST_Util.range = r
+                FStar_Parser_AST_Util.range = r1
               }
         | FStar_Pervasives.Inl id ->
             let splicer =
@@ -37,7 +47,7 @@ let (extension_parser : FStar_Parser_AST_Util.extension_parser) =
                 let uu___1 =
                   FStar_Compiler_List.map lid_as_term
                     ctx.FStar_Parser_AST_Util.open_namespaces in
-                FStar_Parser_AST.mkConsList rng uu___1 in
+                FStar_Parser_AST.mkConsList r uu___1 in
               let abbrevs =
                 let uu___1 =
                   FStar_Compiler_List.map
@@ -48,13 +58,40 @@ let (extension_parser : FStar_Parser_AST_Util.extension_parser) =
                              let uu___3 = FStar_Ident.string_of_id a in
                              str uu___3 in
                            let m1 = lid_as_term m in
-                           FStar_Parser_AST.mkTuple [a1; m1] rng)
+                           FStar_Parser_AST.mkTuple [a1; m1] r)
                     ctx.FStar_Parser_AST_Util.module_abbreviations in
-                FStar_Parser_AST.mkConsList rng uu___1 in
-              FStar_Parser_AST.mkApp head
-                [(namespaces, FStar_Parser_AST.Nothing);
-                (abbrevs, FStar_Parser_AST.Nothing);
-                ((str contents), FStar_Parser_AST.Nothing)] rng in
+                FStar_Parser_AST.mkConsList r uu___1 in
+              let uu___1 =
+                let line =
+                  let uu___2 = FStar_Compiler_Range_Ops.start_of_range r in
+                  FStar_Compiler_Range_Ops.line_of_pos uu___2 in
+                let col =
+                  let uu___2 = FStar_Compiler_Range_Ops.start_of_range r in
+                  FStar_Compiler_Range_Ops.col_of_pos uu___2 in
+                let uu___2 = FStar_Compiler_Range_Ops.file_of_range r in
+                (uu___2, line, col) in
+              match uu___1 with
+              | (file_name, line, col) ->
+                  let uu___2 =
+                    let uu___3 =
+                      let uu___4 =
+                        let uu___5 =
+                          let uu___6 =
+                            let uu___7 =
+                              let uu___8 = i line in
+                              (uu___8, FStar_Parser_AST.Nothing) in
+                            let uu___8 =
+                              let uu___9 =
+                                let uu___10 = i col in
+                                (uu___10, FStar_Parser_AST.Nothing) in
+                              [uu___9] in
+                            uu___7 :: uu___8 in
+                          ((str file_name), FStar_Parser_AST.Nothing) ::
+                            uu___6 in
+                        ((str contents), FStar_Parser_AST.Nothing) :: uu___5 in
+                      (abbrevs, FStar_Parser_AST.Nothing) :: uu___4 in
+                    (namespaces, FStar_Parser_AST.Nothing) :: uu___3 in
+                  FStar_Parser_AST.mkApp head uu___2 r in
             let uu___1 =
               let uu___2 =
                 let uu___3 =
@@ -62,5 +99,42 @@ let (extension_parser : FStar_Parser_AST_Util.extension_parser) =
                 (true, uu___3, splicer) in
               FStar_Parser_AST.Splice uu___2 in
             FStar_Pervasives.Inr uu___1
-let (uu___26 : unit) =
+let (uu___34 : unit) =
   FStar_Parser_AST_Util.register_extension_parser "pulse" extension_parser
+let (parse_pulse :
+  FStar_TypeChecker_Env.env ->
+    Prims.string Prims.list ->
+      (Prims.string * Prims.string) Prims.list ->
+        Prims.string ->
+          Prims.string ->
+            Prims.int ->
+              Prims.int ->
+                (PulseSyntaxWrapper.st_term,
+                  (Prims.string * FStar_Compiler_Range_Type.range))
+                  FStar_Pervasives.either)
+  =
+  fun env ->
+    fun namespaces ->
+      fun module_abbrevs ->
+        fun content ->
+          fun file_name ->
+            fun line ->
+              fun col ->
+                let namespaces1 =
+                  FStar_Compiler_List.map FStar_Ident.path_of_text namespaces in
+                let module_abbrevs1 =
+                  FStar_Compiler_List.map
+                    (fun uu___ ->
+                       match uu___ with
+                       | (x, l) ->
+                           let uu___1 = FStar_Ident.path_of_text l in
+                           (x, uu___1)) module_abbrevs in
+                let env1 =
+                  PulseDesugar.initialize_env env namespaces1 module_abbrevs1 in
+                let range =
+                  let p = FStar_Compiler_Range_Type.mk_pos line col in
+                  FStar_Compiler_Range_Type.mk_range file_name p p in
+                let uu___ = Pulse_Parser.parse_decl content range in
+                match uu___ with
+                | FStar_Pervasives.Inl d -> PulseDesugar.desugar_decl env1 d
+                | FStar_Pervasives.Inr e -> FStar_Pervasives.Inr e
